Many Counting lemmas

theories/algebra/Counting.ec
@@ -23,33 +23,31 @@ proof. by move => P_ IH n /ltzE; apply/le_ind => // {n} n /ltzE; apply/IH. qed.
 
 lemma strong_ind P :
   P 0 =>
-  (forall n , (forall k , k \in range 0 n => P k) => P n) =>
+  (forall n , 0 <= n => (forall k , k \in range 0 n => P k) => P n) =>
   (forall n , 0 <= n => P n).
 proof.
   move => P0 IHS n le0n; elim: n le0n {1 2 4}n (le0n) (lerr n) => [|n le0n IHn] k.
   + by move => le0k lek0; move: (eqz_leq k 0); rewrite lek0 le0k /= => ->>.
   move => le0k /ler_eqVlt [->> {le0k}|/ltzS]; [|by apply/IHn].
-  by apply/IHS => k /mem_range [le0k /ltzS lekn]; apply/IHn.
+  by apply/IHS; [apply/addr_ge0|move => k /mem_range [le0k /ltzS lekn]; apply/IHn].
 qed.
 
 lemma le_strong_ind P (m : int) :
   P m =>
-  (forall n , (forall k , k \in range m n => P k) => P n) =>
+  (forall n , m <= n => (forall k , k \in range m n => P k) => P n) =>
   (forall n , m <= n => P n).
 proof.
-  move => Pm IH n /subr_ge0 le0_; rewrite -(subrK n m).
-  move: (n - m) le0_ => +; move => {n} n le0n.
-  pose Q n:= P (n + m); apply/(strong_ind Q) => //.
-  move => {n le0n} n IHn; rewrite /(Q _); apply/IH.
-  move => k mem_; rewrite -(subrK k m); apply/IHn.
-  by apply/mem_range_subr.
+  move => Pm IH n /subr_ge0 le0_; rewrite -(subrK n m); move: (n - m) le0_ => +.
+  move => {n} n le0n; pose Q n:= P (n + m); apply/(strong_ind Q) => //.
+  move => {n le0n} n le0n IHn; rewrite /(Q _); apply/IH; [by apply/ler_addr|].
+  by move => k mem_; rewrite -(subrK k m); apply/IHn/mem_range_subr.
 qed.
 
 lemma lt_strong_ind P (m : int) :
   P (m + 1) =>
-  (forall n , (forall k , k \in range (m + 1) n => P k) => P n) =>
+  (forall n , m < n => (forall k , k \in range (m + 1) n => P k) => P n) =>
   (forall n , m < n => P n).
-proof. by move => P_ IH n /ltzE; apply/le_strong_ind. qed.
+proof. by move => P_ IH n /ltzE; apply/le_strong_ind => // ? /ltzE; apply/IH. qed.
 
 lemma add_ind P :
   P 1 =>
@@ -57,24 +55,23 @@ lemma add_ind P :
   (forall n , 0 < n => P n).
 proof. by move => P1 IHA; apply/lt_ind => // n lt0n Pn; apply/IHA. qed.
 
-(*TODO: move*)
-lemma prime2 :
-  prime 2.
-proof. by apply/primeP => /=; rewrite range_ltn // range_geq. qed.
-
 lemma compositeP n :
   1 < n =>
   ! prime n =>
   exists a b , 1 < a /\ 1 < b /\ n = a * b.
 proof.
-  move => lt1n; apply/contraR; rewrite negb_exists /= => forall_.
-  apply/primeP; split => // a mem_; rewrite /coprime eq_sym.
-  apply/gcd_uniq => //=; [by rewrite negb_and gtr_eqF // ltzE ltzW|].
-  move => y /dvdzP [x] ->> dvdya; move/(_ x): forall_.
-  rewrite negb_exists /= => /(_ y) /= /negb_and; rewrite -!lerNgt.
-  case => //; apply/contraLR; rewrite -!ltrNge.
-  (*TODO: issue here*)
-  admit.
+  move => lt1n; rewrite /prime; rewrite lt1n /= negb_forall /=.
+  case => a; rewrite negb_imply negb_or => -[dvdan] [neq_1 neq_n].
+  exists `|a| (n %/ `|a|); rewrite mulrC divzE modz_abs !ltrNge.
+  move/dvdzE: (dvdan) => -> /=; rewrite -negb_or !ler_norml.
+  rewrite !le2_mem_range /= 3?range_ltn //= range_geq //=.
+  apply/negP; case => [[|[|]] ->> //=|]; [by move/dvd0z: dvdan => ->>|].
+  rewrite lez_divLR ?dvdzE ?modz_abs -?dvdzE //= ?ltrNge.
+  + apply/negP => le_0; move: (eqz_leq 0 `|a|); rewrite le_0 normr_ge0 /=.
+    by rewrite eq_sym normr0P; apply/negP => ->>; move/dvd0z: dvdan => ->>.
+  move: (dvdz_le _ _ _ dvdan); [by apply/gtr_eqF/ltzE/ltzW|].
+  rewrite (ger0_norm n); [by apply/ltzW/ltzE/ltzW|move => ?; apply/negP => ?].
+  by move: neq_n; rewrite eqz_leq /=; split.
 qed.
 
 lemma mul_ind P :
@@ -82,11 +79,13 @@ lemma mul_ind P :
   (forall m n , 1 < m => 1 < n => P m => P n => P (m * n)) =>
   (forall n , 1 < n => P n).
 proof.
-  move => Pp IHM; apply/lt_strong_ind => /=.
-  + by apply/Pp/prime2.
-  move => n IHn; case: (prime n) => [prime_n|Nprime_n]; [by apply/Pp|].
-  search _ (!prime _).
-  admit.
+  move => Pp IHM; apply/lt_strong_ind => /=; [by apply/Pp/prime2|].
+  move => n lt1n IHn; case: (prime n) => [prime_n|Nprime_n]; [by apply/Pp|].
+  case: (compositeP _ lt1n Nprime_n) => a b [lt1a] [lt1b] ->>; apply/IHM => //.
+  + apply/IHn/mem_range; rewrite -ltzS -ltr_subl_addr lt1a /=; apply/subr_gt0.
+    by rewrite -mulN1r mulrC -mulrDl; apply/mulr_gt0; [apply/subr_gt0|apply/ltzE/ltzW].
+  apply/IHn/mem_range; rewrite -ltzS -ltr_subl_addr lt1b /=; apply/subr_gt0.
+  by rewrite -mulN1r -mulrDl; apply/mulr_gt0; [apply/subr_gt0|apply/ltzE/ltzW].
 qed.
 
 lemma coprime_ind P :
@@ -94,30 +93,70 @@ lemma coprime_ind P :
   (forall m n , 1 < m => 1 < n => coprime m n => P m => P n => P (m * n)) =>
   (forall n , 1 < n => P n).
 proof.
-  admit.
+  move => Ppp IHM; apply/lt_strong_ind => /=; [by move: (Ppp _ 1 prime2 _); rewrite // expr1|].
+  move => n lt1n IHn; case: (pow_prime_divisors n _); [by apply/ltzE/ltzW|].
+  case => [/is_ppdec_nil ->> //|[p k] pps /is_ppdec_cons |> [prime_p _] lt0k dvd_ Ndvd_ _].
+  case (n = p ^ k) => [->>|neq]; [by apply/Ppp|]; rewrite -(divzK _ _ dvd_); apply/IHM.
+  + apply/ltz_divRL => //=; [by apply/expr_gt0/gt0_prime|].
+    move: (dvdz_le _ _ _ dvd_); [by apply/gtr_eqF/ltzE/ltzW|].
+    rewrite gtr0_norm; [by apply/expr_gt0/gt0_prime|]; rewrite gtr0_norm; [by apply/ltzE/ltzW|].
+    by move => /ler_eqVlt; rewrite eq_sym neq.
+  + apply/(ltr_le_trans p); [by apply/gt1_prime|]; rewrite -{1}expr1.
+    by apply/ler_weexpn2l => /=; [apply/ltzW/gt1_prime|move/ltzE: lt0k].
+  + admit.
+  + apply/IHn/mem_range; rewrite ltz_divLR; [by apply/expr_gt0/gt0_prime|].
+    rewrite -subr_gt0 -mulN1r mulrC -mulrDl mulr_gt0 /=; [|by apply/ltzE/ltzW| ].
+    - apply/subr_gt0/(ltr_le_trans p); [by apply/gt1_prime|]; rewrite -{1}expr1.
+      by apply/ler_weexpn2l => /=; [apply/ltzW/gt1_prime|move/ltzE: lt0k].
+    apply/ltzS/ltr_subl_addr/ltz_divRL => //=; [by apply/expr_gt0/gt0_prime|].
+    move: (dvdz_le _ _ _ dvd_); [by apply/gtr_eqF/ltzE/ltzW|].
+    rewrite gtr0_norm; [by apply/expr_gt0/gt0_prime|]; rewrite gtr0_norm; [by apply/ltzE/ltzW|].
+    by move => /ler_eqVlt; rewrite eq_sym neq.
+  apply/IHn/mem_range; move: (dvdz_le _ _ _ dvd_); [by apply/gtr_eqF/ltzE/ltzW|].
+  rewrite gtr0_norm; [by apply/expr_gt0/gt0_prime|]; rewrite gtr0_norm; [by apply/ltzE/ltzW|].
+  move => /ler_eqVlt; rewrite eq_sym neq /= => -> /=; apply/ltzS/ltr_subl_addr => /=.
+  apply/(ltr_le_trans p); [by apply/gt1_prime|]; rewrite -{1}expr1.
+  by apply/ler_weexpn2l => /=; [apply/ltzW/gt1_prime|move/ltzE: lt0k].
 qed.
 
 
 (* ==================================================================== *)
-op coprimes n = filter (coprime n) (range 1 n).
+op coprimes n = filter (coprime n) (range 1 (n + 1)).
 
 lemma coprimesP n k :
-  k \in coprimes n <=> (coprime n k /\ k \in range 1 n).
+  k \in coprimes n <=> (coprime n k /\ k \in range 1 (n + 1)).
 proof. by rewrite mem_filter. qed.
 
 lemma coprimes_nil n :
-  n <= 1 =>
+  n <= 0 =>
   coprimes n = [].
-proof. by move => ?; rewrite /coprimes range_geq. qed.
+proof. by move => ?; rewrite /coprimes range_geq // -ler_subr_addr. qed.
 
-lemma coprimes1 n :
-  1 < n <=> 1 \in coprimes n.
-proof. by rewrite coprimesP /coprime gcdz1 /= mem_range. qed.
+lemma coprimes1 :
+  coprimes 1 = [1].
+proof. by rewrite /coprimes range_ltn // range_geq. qed.
+
+lemma coprimes_mem1 n :
+  1 <= n <=> 1 \in coprimes n.
+proof. by rewrite coprimesP /coprime gcdz1 /= mem_range ltzS. qed.
+
+lemma coprimes_subseq n :
+  1 < n =>
+  subseq (coprimes n) (range 1 n).
+proof.
+  move => lt1n; rewrite /coprimes rangeSr ?ltzW //.
+  rewrite filter_rcons /coprime.
+  admit.
+qed.
 
 lemma coprimes_prime p :
   prime p =>
   coprimes p = range 1 p.
-proof. by move => /primeP [lt1p mem_]; rewrite /coprimes eq_in_filter_predT. qed.
+proof.
+  move => /primeP [lt1p mem_]; rewrite /coprimes rangeSr ?ltzW //.
+  rewrite filter_rcons eq_in_filter_predT // /coprime.
+  admit.
+qed.
 
 lemma coprimes_pow_prime p n :
   prime p =>
@@ -136,22 +175,27 @@ lemma phi_ge0 n :
 proof. by apply/size_ge0. qed.
 
 lemma phi_eq0 n :
-  n <= 1 =>
+  n <= 0 =>
   phi n = 0.
 proof. by move => len0; rewrite /phi coprimes_nil. qed.
 
+lemma phi1 :
+  phi 1 = 1.
+proof. by rewrite /phi coprimes1. qed.
+
 lemma phi_gt0 n :
-  1 < n =>
+  1 <= n =>
   0 < phi n.
-proof. by rewrite /phi -has_predT hasP => /coprimes1 ?; exists 1; rewrite /predT. qed.
+proof. by rewrite /phi -has_predT hasP => /coprimes_mem1 ?; exists 1; rewrite /predT. qed.
 
 lemma phi_ltid n :
-  0 < n =>
+  1 < n =>
   phi n < n.
 proof.
-move => le0n; rewrite /phi /coprimes; apply/(ler_lt_trans (size (range 1 n))).
-+ by apply/le_size_filter.
-by rewrite size_range ler_maxr; [rewrite -ltzS|rewrite ltzE].
+move => /coprimes_subseq; rewrite /phi.
+(*TODO: missing*)
+search _ subseq size.
+admit.
 qed.
 
 lemma phi_prime p :
@@ -173,6 +217,7 @@ qed.
 lemma phi_coprime m n :
   0 < m =>
   0 < n =>
+  coprime m n =>
   phi (m * n) = phi m * phi n.
 proof.
   admit.
@@ -210,7 +255,7 @@ qed.
 lemma divisors_pow_prime p n :
   prime p =>
   0 <= n =>
-  divisors (p ^ n) = map (exp p) (range 0 n).
+  divisors (p ^ n) = map (exp p) (range 0 (n + 1)).
 proof.
   admit.
 qed.
@@ -226,23 +271,18 @@ qed.
 
 lemma sum_phi n :
   0 < n =>
-  big predT phi (divisors n) = n - 1.
+  big predT phi (divisors n) = n.
 proof.
-  case/ltzE/ler_eqVlt => [<<-|/=]; [by rewrite divisors1 big_seq1 phi_eq0|].
-  pose P n:= big predT phi (divisors n) = n - 1; apply/(coprime_ind P); rewrite /P => {P}.
+  case/ltzE/ler_eqVlt => [<<-|/=]; [by rewrite divisors1 big_seq1 phi1|].
+  pose P n:= big predT phi (divisors n) = n; apply/(coprime_ind P); rewrite /P => {P}.
   + move => p k prime_p lt0k; rewrite divisors_pow_prime ?ltzW // big_mapT.
-    rewrite big_ltn // {1}/(\o) expr0 phi_eq0 //=.
+    rewrite big_ltn; [by apply/addr_gt0|]; rewrite {1}/(\o) expr0 phi1 //=.
     rewrite (eq_big_int _ _ _ (fun n => p ^ n - p ^ (n - 1))).
     - by move => ? [?] _; rewrite /(\o) /= phi_pow_prime // ltzE.
-    rewrite -sumrB; move: (range_add 0 (k - 1) 1) => /= {2}->.
+    rewrite -sumrB; move: (range_add 0 k 1) => /= {2}->.
     rewrite big_mapT (eq_big_int 0 _ _ ((^) p)); [by move => ?|].
-    case/ltzE/ler_eqVlt: lt0k => [<<-/=|/= lt1k].
-    - rewrite !big_geq // expr1.
-      admit.
-    rewrite (big_ltn 0) ?ltzS ?subr_gt0 // expr0 opprD addrA addrAC /=.
-    move: (rangeSr 1 (k - 1) _) => /=; [by apply/ltzS|move => ->].
-    rewrite big_rcons {1}/predT /= (addrAC _ (p ^ _)) /=.
-    search _ (_ _ + big _ _ (range _ _)).
-    admit.
+    rewrite (big_ltn 0) // expr0 opprD !addrA (addrAC 1) /=.
+    move: (rangeSr 1 k _) => /=; [by move/ltzE: lt0k|move => ->].
+    by rewrite big_rcons {1}/predT /= addrAC.
   admit.
 qed.
